theories/typing/bool.v
@@ -1,4 +1,3 @@
-From iris.proofmode Require Import tactics.
 From lrust.typing Require Export type.
 (* From lrust.typing Require Import programs. *)
 Set Default Proof Using "Type".
