theories/typing/int.v
@@ -1,4 +1,3 @@
-From iris.proofmode Require Import tactics.
 From lrust.typing Require Export type.
 From lrust.typing Require Import bool (* programs *).
 Set Default Proof Using "Type".
