theories/typing/mod_ty.v
@@ -1,4 +1,3 @@
-From iris.proofmode Require Import tactics.
 From lrust.util Require Import basic.
 From lrust.typing Require Export type.
 Set Default Proof Using "Type".
