theories/typing/product.v
@@ -1,7 +1,4 @@
 Require Import FunctionalExtensionality Equality.
-From iris.proofmode Require Import tactics.
-From iris.algebra Require Import list numbers.
-From lrust.util Require Import basic update types.
 From lrust.typing Require Export type.
 From lrust.typing Require Import lft_contexts mod_ty.
 
