theories/util/update.v
@@ -8,6 +8,9 @@ Section lemmas.
 Context `{BiFUpd PROP}.
 Implicit Type P Q: PROP.
 
+Global Instance step_fupdN_proper E n : Proper ((⊣⊢) ==> (⊣⊢)) (λ P, |={E}▷=>^n P)%I.
+Proof. by elim n; [apply _|]=>/= *??->. Qed.
+
 Lemma step_fupdN_nmono E m n P : m ≤ n → (|={E}▷=>^m P) -∗ (|={E}▷=>^n P).
 Proof.
   move: n. elim m=>/= [|?]; [iIntros; by iApply step_fupdN_intro|].
